theories/Misc/Take.v
@@ -1,8 +1,7 @@
 (*|
 ======================================================
-Take N visible steps from a ctree and return the rest.
+Methods and lemmas for splitting ctrees
 ======================================================
-A generalization of [head]
 
 .. coq:: none
 |*)
@@ -15,87 +14,117 @@ From CTree Require Import
 Set Implicit Arguments.
 Set Contextual Implicit.
 
-(*| This function extracts "at most" [n] visible steps from the ctree
-   and puts the rest as the return value to be continued later. |*)
-Fixpoint take{E C X}(n: nat): ctree E C X -> ctree E C (ctree E C X) :=
-  cofix F (t: ctree E C X): ctree E C (ctree E C X) :=
+Section Take.
+  Context {E C: Type -> Type} {X: Type}.
+
+  (*| This function extracts "at most" [n] visible steps from the ctree
+    and puts the rest as the return value to be continued later. |*)
+  Fixpoint take(n: nat): ctree E C X -> ctree E C (ctree E C X) :=
+    cofix F (t: ctree E C X): ctree E C (ctree E C X) :=
+      match n with
+      | 0 => Ret t
+      | S m => 
+          match observe t with
+          | RetF x => Ret (Ret x)
+          | VisF e k => Vis e (fun i => take m (k i))        (* inductive step *)
+          | BrSF c k => Br true c (fun i => take m (k i))    (* inductive step *)
+          | BrDF c k => Br false c (fun i => F (k i))        (* coinductive, could spin in delay loop *)
+          end
+      end.
+
+  Notation take_ n t :=
     match n with
     | 0 => Ret t
     | S m => 
         match observe t with
         | RetF x => Ret (Ret x)
-        | VisF e k => Vis e (fun i => take m (k i))        (* inductive step *)
-        | BrSF c k => Br true c (fun i => take m (k i))    (* inductive step *)
-        | BrDF c k => Br false c (fun i => F (k i))        (* coinductive, could spin in delay loop *)
+        | VisF e k => Vis e (fun i => take m (k i))
+        | BrSF c k => Br true c (fun i => take m (k i))
+        | BrDF c k => Br false c (fun i => take n (k i))
         end
     end.
+  
+  Lemma unfold_take : forall (n: nat) (t : ctree E C X),
+      take n t ≅ take_ n t.
+  Proof.
+    intro n; induction n; intro; step; eauto.
+  Qed.
+  
+  (*| Taking 0 visible steps returns the unchanged ctree |*)
+  Lemma unfold_0_take : forall (t: ctree E C X),
+      take 0 t ≅ Ret t.
+  Proof.
+    setoid_rewrite unfold_take; reflexivity.
+  Qed.
 
-Notation take_ n t :=
-  match n with
-  | 0 => Ret t
-  | S m => 
+  Lemma unfold_Sn_take : forall (t: ctree E C X) n,
+      take (S n) t ≅ match observe t with
+                     | RetF x => Ret (Ret x)
+                     | VisF e k => Vis e (fun i => take n (k i))
+                     | BrSF c k => Br true c (fun i => take n (k i))
+                     | BrDF c k => Br false c (fun i => take (S n) (k i))
+                     end.
+  Proof. setoid_rewrite unfold_take; reflexivity. Qed.  
+
+  (* Nice educational proof *)
+  #[global] Instance equ_eq_take_proper {n}:
+    Proper (equ eq ==> equ (equ eq)) (take n).
+  Proof.
+    unfold Proper, respectful.
+    revert n.  
+    coinduction ? ?.
+    intro n; destruct n; intros.
+    - rewrite !unfold_0_take; auto; now econstructor.
+    - rewrite !unfold_take; step in H0; inv H0.
+      + now constructor.
+      + constructor; intros; auto.
+      + destruct b; econstructor; auto. 
+  Qed.
+
+End Take.
+
+(*| Traverse the ctree until you encounted a blocking Vis node, then split right before it. |*)
+Section ToBlocked.
+  Context {E C: Type -> Type} {X: Type}.
+  Context (is_blocking: forall T, E T -> bool).
+  
+  Definition to_blocked: ctree E C X -> ctree E C (ctree E C X) :=
+    cofix F (t: ctree E C X): ctree E C (ctree E C X) :=
       match observe t with
       | RetF x => Ret (Ret x)
-      | VisF e k => Vis e (fun i => take m (k i))
-      | BrSF c k => Br true c (fun i => take m (k i))
-      | BrDF c k => Br false c (fun i => take n (k i))
-    end
-  end.
+      | VisF e k =>
+          if is_blocking e then (Ret (Vis e k))
+          else (Vis e (fun i => F (k i)))
+      | BrSF c k => BrS c (fun i => F (k i))
+      | BrDF c k => BrD c (fun i => F (k i))
+      end.
 
+  Notation to_blocked_ t := 
+    match observe t with
+    | RetF x => Ret (Ret x)
+    | VisF e k =>
+        if is_blocking e then (Ret (Vis e k))
+        else (Vis e (fun i => to_blocked (k i)))
+    | BrSF c k => BrS c (fun i => to_blocked (k i))
+    | BrDF c k => BrD c (fun i => to_blocked (k i))
+    end.
 
-(*| Re-attach heads after [take] |*)
-(* Definition flatten {E C X} (u: ctree E C (ctree E C X)) :=
-  CTree.bind u (fun x => x).
- *)
+  Lemma unfold_to_blocked : forall (t : ctree E C X),
+      to_blocked t ≅ to_blocked_ t.
+  Proof. intro; step; eauto. Qed.
+End ToBlocked.
+
+(*| Re-attach split ctrees |*)
 Notation flatten u := (CTree.bind u (fun x => x)) (only parsing).
 
-Lemma unfold_take {E C X} : forall (n: nat) (t : ctree E C X),
-    take n t ≅ take_ n t.
-Proof.
-  intro n; induction n; intro; step; eauto.
-Qed.
-
-(*| Taking 0 visible steps returns the unchanged ctree |*)
-Lemma unfold_0_take {E C X} : forall (t: ctree E C X),
-    take 0 t ≅ Ret t.
-Proof.
-  setoid_rewrite unfold_take; reflexivity.
-Qed.
-
-Lemma unfold_Sn_take {E C X}: forall (t: ctree E C X) n,
-    take (S n) t ≅ match observe t with
-                   | RetF x => Ret (Ret x)
-                   | VisF e k => Vis e (fun i => take n (k i))
-                   | BrSF c k => Br true c (fun i => take n (k i))
-                   | BrDF c k => Br false c (fun i => take (S n) (k i))
-                   end.
-Proof.
-  setoid_rewrite unfold_take; reflexivity.
-Qed.  
-
-(* Nice educational proof *)
-#[global] Instance equ_eq_take_proper {E C X n}:
-  Proper (equ eq ==> equ (equ eq)) (@take E C X n).
-Proof.
-  unfold Proper, respectful.
-  revert n.  
-  coinduction ? ?.
-  intro n; destruct n; intros.
-  - rewrite !unfold_0_take; auto; now econstructor.
-  - rewrite !unfold_take; step in H0; inv H0.
-    + now constructor.
-    + constructor; intros; auto.
-    + destruct b; econstructor; auto. 
-Qed.
-
-(* LEF: Must find a way to generalize [bind_equ_cong] to [equ (equ eq)] like here. *)
 #[global] Instance bind_equ_equ_cong :
   forall (E B : Type -> Type) (X Y : Type) (R : rel Y Y) RR,
-    Proper (equ (equ (@eq X)) ==> pointwise_relation (ctree E B X) (et R RR) ==> et R RR) (@CTree.bind E B (ctree E B X) Y).
+    Proper (equ (equ (@eq X)) ==> pointwise (equ eq) (et R RR) ==> et R RR)
+           (@CTree.bind E B (ctree E B X) Y).
 Proof.
-  repeat red; cbn; intros.
+  repeat red; intros.
   eapply et_clo_bind; eauto.
-Admitted.
+Qed. 
 
 Lemma take_flatten_id {E C X}: forall n (t: ctree E C X),
     flatten (take n t) ≅ t.
@@ -103,11 +132,13 @@ Proof.
   Opaque take.
   coinduction ? CIH; intros; destruct n.
   - rewrite unfold_0_take, bind_ret_l; auto.
-  - rewrite (ctree_eta t); rewrite unfold_take; desobs t; cbn.
-    + now rewrite bind_ret_l.
-    + rewrite bind_vis.
+  - rewrite unfold_take.
+    assert(Ht: t ≅ {| _observe := observe t |}) by (apply ctree_eta).
+    desobs t.
+    + rewrite bind_ret_l; now rewrite Ht.
+    + rewrite bind_vis, Ht.
       now econstructor.
-    + destruct vis; rewrite bind_br; econstructor; intros; eauto.
+    + destruct vis; rewrite bind_br; rewrite Ht; econstructor; intros; eauto.
 Qed.
 
 (* This is the [Ret (Ret x)] on RHS *)
