theories/Logic/Kripke.v
@@ -1,0 +1,228 @@
+(*|
+=========================================
+Modal logics over ctrees
+=========================================
+|*)
+
+From ITree Require Import
+     Events.State
+     CategoryOps.
+
+From CTree Require Import
+     Eq
+     CTree
+     Interp.Par
+     FoldStateT.
+
+From Coq Require Import
+     Classes.SetoidClass
+     Classes.RelationPairs.
+
+Import CTreeNotations.
+
+Set Implicit Arguments.
+
+(* From ctree labels to kripke states *)
+Class Handler (E: Type -> Type) (S: Type) := {
+    hfold: forall X, E X -> X -> S -> S;
+  }.
+
+#[global] Instance Handler_state S: Handler (stateE S) S :=
+  {|
+    hfold _ e _ s :=
+    match e with
+    | Put s => s
+    | Get _ => s
+    end
+  |}.
+
+#[global] Instance Handler_par: Handler parE nat := 
+  {| hfold _ e _ s := match e with Switch i => i end |}.
+
+(* WHY this loops during instance resolution *)
+#[global] Instance Handler_plus{E F: Type -> Type}{S T}
+ (h: Handler E S) (g: Handler F T) : Handler (E+'F) (S*T) :=
+  {|
+    hfold _ ef x '(s,t) := 
+    match ef with
+    | inl1 e => (h.(hfold) e x s, t)
+    | inr1 f => (s, g.(hfold) f x t)
+    end
+  |}.
+
+Section Kripke.
+  Context {E C: Type -> Type} {X S: Type}
+          {h: Handler E S} {HasStuck: B0 -< C}.
+
+  (* Kripke state predicates *)
+  Notation SP := (ctree E C X -> S -> Prop).
+    
+  (* Kripke transition given a handler *)
+  Variant ktrans: (ctree E C X * S) -> (ctree E C X * S) -> Prop :=
+    | kTau (t u: ctree E C X) (s: S):
+      trans tau t u ->
+      ktrans (t, s) (u, s)
+    | kVis (t u: ctree E C X) {Y} (x: Y) (e: E Y) (s: S):
+      trans (obs e x) t u ->
+      ktrans (t, s) (u, h.(hfold) e x s)
+             
+    | kRet (t u: ctree E C X) (x: X) (s: S):
+      trans (val x) t stuckD ->
+      u ≅ Ret x ->
+      ktrans (t, s) (u, s).
+
+  Hint Constructors ktrans: core.
+
+  #[global] Instance proper_ktrans_equ:
+    Proper (equ eq * eq ==> equ eq * eq ==> iff) ktrans.
+  Proof.
+    unfold Proper, respectful, impl; cbn.
+    intros [t s] [u x] [EQt ?] [t' s'] [u' x'] [EQt' H3]; simpl in *.
+    unfold RelCompFun in *; cbn in *; subst.    
+    split; intro H; inv H.
+    - rewrite EQt, EQt' in H1.
+      now apply kTau.
+    - rewrite EQt, EQt' in H1.
+      now apply kVis.
+    - apply kRet with x0; [now rewrite <- EQt | now rewrite <- EQt'].
+    - rewrite <- EQt, <- EQt' in H1.
+      now apply kTau.
+    - rewrite <- EQt, <- EQt' in H1.
+      now apply kVis.
+    - apply kRet with x0; [now rewrite EQt | now rewrite EQt'].
+  Qed.
+
+  Lemma trans_val_sbisim: forall (t u: ctree E C X) (x: X),
+      trans (val x) t stuckD ->
+      t ~ u ->
+      trans (val x) u stuckD.
+  Proof.
+    intros.    
+    unfold trans, transR in H; cbn in H.
+    remember (val x).
+    induction H; intros; eauto; try solve [inv Heql].
+    (* Ah lost [observe t] *)
+  Admitted.
+
+  Lemma ktrans_sbisim_l: forall (t1 t2 t1': ctree E C X) s s',
+      ktrans (t1,s) (t1',s') ->
+      t1 ~ t2 ->
+      exists t2', ktrans (t2,s) (t2',s') /\ t1' ~ t2'.
+  Proof.
+    intros * TR  Hsb.
+    inv TR; intros.
+    1,2: step in Hsb; apply Hsb in H0 as (l2 & t2' & TR2 & ? & <-); exists t2'; split; eauto.
+    exists (Ret x); rewrite H4; split; eauto.
+    apply kRet with x; [| reflexivity]. 
+    now apply trans_val_sbisim with (u:=t2) in H2.
+  Qed.
+
+  (*| Invert [ktrans] |*)
+  Ltac shallow_inv_ktrans H := dependent destruction H; try solve [inv H];
+                               intuition; unfold trans,transR in H; cbn in H;
+                               dependent destruction H;
+                               repeat change (CTree.subst ?k ?t) with (CTree.bind t k) in H;
+                               repeat lazymatch goal with
+                                      | H: ?t |- ?t => exact H
+                                      | H: observe ?t = observe ?u |- _ => apply observe_equ_eq in H
+                                      end.
+
+  Lemma ktrans_ret: forall x (t t': ctree E C X) s s',
+      ktrans (Ret x, s) (t', s') <->
+      t' ≅ Ret x /\ s = s'.
+  Proof.
+    split; intros.
+    - shallow_inv_ktrans H.
+    - destruct H as (-> & ->); eapply kRet; eauto; econstructor.
+  Qed.
+
+  Lemma ktrans_tau_inv: forall c (t': ctree E C X) (k: X -> ctree E C X) s s',
+      ktrans (BrS c k, s) (t', s') ->
+      exists x, t' ≅ k x /\ s = s'.
+  Proof.
+    intros.
+    shallow_inv_ktrans H.
+    exists x0; rewrite <- x; intuition.
+  Qed.
+  
+  Lemma ktrans_tau_goal: forall c x (t': ctree E C X) (k: X -> ctree E C X) s s',
+      t' ≅ k x /\ s = s' ->
+      ktrans (BrS c k, s) (t', s').
+  Proof.
+    intros.
+    destruct H as (-> & ->).
+    apply kTau; econstructor; eauto.
+  Qed.
+
+  Lemma ktrans_vis_inv: forall e (t': ctree E C X) (k: X -> ctree E C X) s s',
+      ktrans (Vis e k, s) (t', s') ->
+      exists x, t' ≅ k x /\ s' = h.(hfold) e x s.
+  Proof.
+    intros.
+    shallow_inv_ktrans H.
+    exists x0; rewrite <- x; intuition.
+  Qed.
+  
+  Lemma ktrans_vis_goal: forall e x (t': ctree E C X) (k: X -> ctree E C X) s s',
+      t' ≅ k x /\ s' = h.(hfold) e x s ->
+      ktrans (Vis e k, s) (t', s').
+  Proof.
+    intros.
+    destruct H as (-> & ->).
+    apply kVis; econstructor; eauto.
+  Qed.
+
+  Lemma ktrans_trigger_inv: forall {Y: Type} (e: E Y) u (k: Y -> ctree E C X) s s',
+      ktrans (trigger e >>= k, s) (u, s') ->
+      exists x, u ≅ k x /\ s' = h.(hfold) e x s.
+  Proof.
+    intros.
+    shallow_inv_ktrans H.
+    rewrite bind_ret_l in H.
+    exists x0.
+    rewrite x in H.
+    intuition.
+  Qed.
+
+
+End Kripke.
+
+Definition is_ret{E C X}(t: ctree E C X): Prop :=
+  exists x, t ≅ Ret x.
+  
+Lemma ktrans_bind_inv: forall {E C X Y S} `{Handler E S} `{B0 -< C} (s s': S)
+                         (t: ctree E C Y) (u: ctree E C X) (k: Y -> ctree E C X),
+    ktrans (x <- t ;; k x, s) (u, s') ->
+    ~ is_ret t /\ (exists t', ktrans (t, s) (t', s') /\ u ≅ x <- t' ;; k x) \/
+      (exists x, ktrans (t, s) (Ret x, s) /\ ktrans (k x, s) (u, s')).
+Proof.
+  intros.
+  inv H1.
+  - apply trans_bind_inv in H3 as [(HV & t' & TR & EQu) | (x & TRv & TRu)].
+    + left; split.
+      * intro CONTRA; destruct CONTRA as (tc & ?);
+          rewrite H1 in TR; inversion TR.
+      * exists t'; split; auto.
+        now apply kTau.
+    + right; exists x; split.
+      * now apply kRet with x.
+      * now apply kTau.
+  - apply trans_bind_inv in H3 as [(HV & t' & TR & EQu) | (x' & TRv & TRu)].
+    + left; split.
+      * intro CONTRA; destruct CONTRA as (tc & ?);
+          rewrite H1 in TR; inversion TR.
+      * exists t'; split; auto.
+        now apply kVis.
+    + right; exists x'; split.
+      * now apply kRet with x'.
+      * now apply kVis.
+  - apply trans_bind_inv in H5 as [(HV & t' & TR & EQu) | (x' & TRv & TRu)].
+    + now contradiction HV.
+    + right; exists x'; split.
+      * now apply kRet with x'.
+      * rewrite H7.
+        now apply kRet with x.
+Qed.
+
+
+
